changed HML definition to include sets, which requires to change subsequent definitions and lemmas; changed those up to, including trace_lemma

HML_list.thy
@@ -4,31 +4,43 @@ theory HML_list
  Transition_Systems
 
 begin
-datatype ('a)formula_list =
+datatype ('a, 'i)hml =
+TT |
+hml_pos \<open>'a\<close> \<open>('a, 'i)hml\<close> |
+hml_conj "'i set" "'i \<Rightarrow> ('a, 'i) hml" "'i set" "'i \<Rightarrow> ('a, 'i) hml" 
+
+(*datatype ('a)formula_list =
 HML_conj \<open>('a)formula_list list\<close>  \<open>('a)formula_list list\<close>
-| HML_poss \<open>'a\<close> \<open>('a)formula_list\<close>
+| HML_poss \<open>'a\<close> \<open>('a)formula_list\<close>*)
 
 context lts begin
 
-fun HML_semantics :: \<open>'s \<Rightarrow> ('a)formula_list \<Rightarrow> bool\<close>
+primrec hml_semantics :: \<open>'s \<Rightarrow> ('a, 's)hml \<Rightarrow> bool\<close>
+(\<open>_ \<Turnstile> _\<close> [50, 50] 50)
+where
+hml_sem_tt: \<open>(_ \<Turnstile> TT) = True\<close> |
+hml_sem_pos: \<open>(p \<Turnstile> (hml_pos \<alpha> \<phi>)) = (\<exists> q. (p \<mapsto>\<alpha> q) \<and> q \<Turnstile> \<phi>)\<close> |
+hml_sem_conj: \<open>(p \<Turnstile> (hml_conj I \<psi>s J n\<psi>s)) = ((\<forall>i \<in> I. p \<Turnstile> (\<psi>s i)) \<and> (\<forall>j \<in> J. \<not>(p \<Turnstile> (n\<psi>s j))))\<close>
+
+(*
+fun HML_semantics :: \<open>'s \<Rightarrow> ('a)formula_list \<Rightarrow> bool\<close> 
 (\<open>_ \<Turnstile> _\<close> [50, 50] 50)
   where
 HML_sem_conj: \<open>(p \<Turnstile> HML_conj \<Phi> \<Psi>) = 
 (\<forall>\<phi>. (\<phi> \<in> set \<Phi> \<longrightarrow> HML_semantics p  \<phi>) \<and> (\<phi> \<in> set \<Psi> \<longrightarrow> \<not>(HML_semantics p \<phi>)))\<close>
 | HML_sem_poss: \<open>(HML_semantics p (HML_poss \<alpha> \<phi>)) = (\<exists> q. (p \<mapsto>\<alpha> q) \<and> q \<Turnstile> \<phi>)\<close>
-
-find_theorems HML_semantics
+*)
 
 text \<open>Two states are HML equivalent if they satisfy the same formula.\<close>
 definition HML_equivalent :: \<open>'s \<Rightarrow> 's \<Rightarrow> bool\<close> where
-  \<open>HML_equivalent p q \<equiv> (\<forall> \<phi>::('a) formula_list. (p \<Turnstile> \<phi>) \<longleftrightarrow> (q \<Turnstile> \<phi>))\<close>
+  \<open>HML_equivalent p q \<equiv> (\<forall> \<phi>::('a, 's) hml. (p \<Turnstile> \<phi>) \<longleftrightarrow> (q \<Turnstile> \<phi>))\<close>
 
 lemma equiv_der:
   assumes "HML_equivalent p q" "\<exists>p'. p \<mapsto>\<alpha> p'"
   shows "\<exists>p' q'. (HML_equivalent p' q') \<and> q \<mapsto>\<alpha> q'"
-  using assms HML_semantics.simps
+  using assms hml_semantics.simps
   unfolding HML_equivalent_def 
-  by (metis empty_iff list.set(1))
+  by metis
 
 
 text \<open>HML_equivalency is transitive\<close>
@@ -39,7 +51,7 @@ text \<open>
   A formula distinguishes one state from another if its true for the
   first and false for the second.
 \<close>
-abbreviation distinguishes ::  \<open>('a) formula_list \<Rightarrow> 's \<Rightarrow> 's \<Rightarrow> bool\<close> where
+abbreviation distinguishes ::  \<open>('a, 's) hml \<Rightarrow> 's \<Rightarrow> 's \<Rightarrow> bool\<close> where
    \<open>distinguishes \<phi> p q \<equiv> p \<Turnstile> \<phi> \<and> \<not> q \<Turnstile> \<phi>\<close>
 
 lemma hml_equiv_sym:
@@ -50,13 +62,15 @@ text \<open>
   If two states are not HML equivalent then there must be a
   distinguishing formula.
 \<close>
+(*assumes that lts is not empty, kann evtl auch aus \<not> HML_equivalent p q gezeigt werden*)
 lemma hml_distinctions:
+  fixes state::"'s"
   assumes \<open>\<not> HML_equivalent p q\<close>
   shows \<open>\<exists>\<phi>. distinguishes \<phi> p q\<close>
 proof-
-  from assms have "\<not> (\<forall> \<phi>::('a) formula_list. (p \<Turnstile> \<phi>) \<longleftrightarrow> (q \<Turnstile> \<phi>))" 
+  from assms have "\<not> (\<forall> \<phi>::('a, 's) hml. (p \<Turnstile> \<phi>) \<longleftrightarrow> (q \<Turnstile> \<phi>))" 
     unfolding HML_equivalent_def by blast
-  then obtain \<phi>::"('a) formula_list" where "(p \<Turnstile> \<phi>) \<noteq> (q \<Turnstile> \<phi>)" by blast
+  then obtain \<phi>::"('a, 's) hml" where "(p \<Turnstile> \<phi>) \<noteq> (q \<Turnstile> \<phi>)" by blast
   then have "((p \<Turnstile> \<phi>) \<and> \<not>(q \<Turnstile> \<phi>)) \<or> (\<not>(p \<Turnstile> \<phi>) \<and> (q \<Turnstile> \<phi>))"
     by blast
   then show ?thesis
@@ -64,47 +78,56 @@ proof-
     show "distinguishes \<phi> p q \<Longrightarrow> \<exists>\<phi>. distinguishes \<phi> p q" by blast
   next
     assume assm: "\<not> p \<Turnstile> \<phi> \<and> q \<Turnstile> \<phi>"
-    show "\<exists>\<phi>. distinguishes \<phi> p q"
-    proof
-      from assm show "(p \<Turnstile> (HML_conj [] [\<phi>])) \<and> \<not> q \<Turnstile>(HML_conj [] [\<phi>])" using HML_semantics.simps
-        by simp
-    qed
+    define n\<phi> where "n\<phi> \<equiv>(hml_conj ({}::'s set) 
+                          ((\<lambda>x. undefined):: 's \<Rightarrow> ('a, 's) hml) 
+                          {state} 
+                          (\<lambda>j. if j = state then \<phi> else undefined))"
+    have "p \<Turnstile> n\<phi> \<and> \<not> q \<Turnstile> n\<phi>" 
+      unfolding n\<phi>_def
+      using hml_semantics.simps assm
+      by force
+    then show ?thesis
+      by blast
   qed
 qed
 
-end
+end (* context lts *)
 
 (*Trace equiv: T \<in> trace, wenn \<phi> dann auch <a>\<phi>.*)
 (*(\<infinity>, 1, 0, 0, 0, 0)*)
-inductive HML_trace :: "('a)formula_list \<Rightarrow> bool"
+inductive HML_trace :: "('a, 's)hml \<Rightarrow> bool"
   where
-trace_conj: "HML_trace (HML_conj [] [])"|
-trace_pos: "HML_trace (HML_poss \<alpha> \<phi>)" if "HML_trace \<phi>"
+trace_tt : "HML_trace TT" |
+trace_conj: "HML_trace (hml_conj {} \<psi>s {} n\<psi>s)"|
+trace_pos: "HML_trace (hml_pos \<alpha> \<phi>)" if "HML_trace \<phi>"
 
 definition HML_trace_formulas where
 "HML_trace_formulas \<equiv> {\<phi>. HML_trace \<phi>}"
 
 text \<open>translation of a trace to a formula\<close>
 
-fun trace_to_formula :: "'a list \<Rightarrow> ('a)formula_list"
+fun trace_to_formula :: "'a list \<Rightarrow> ('a, 's)hml"
   where
-"trace_to_formula [] = HML_conj [] []" |
-"trace_to_formula (a#xs) = HML_poss a (trace_to_formula xs)"
+"trace_to_formula [] = TT" |
+"trace_to_formula (a#xs) = hml_pos a (trace_to_formula xs)"
 
-inductive HML_failure :: "('a)formula_list \<Rightarrow> bool"
-  where
-trace: "HML_failure (HML_poss \<alpha> \<phi>)" if "HML_failure \<phi>" |
-neg: "HML_failure (HML_conj [] x2)" if "\<forall>y \<in> (set x2). \<exists>\<alpha>. y = HML_poss \<alpha> (HML_conj [] [])" 
+(*
 
-inductive HML_simulation :: "('a)formula_list \<Rightarrow> bool"
+inductive HML_failure :: "('a, 's)hml \<Rightarrow> bool"
   where
-sim_pos: "HML_simulation (HML_poss \<alpha> \<phi>)" if "HML_simulation \<phi>"|
-sim_conj: "HML_simulation (HML_conj xs [])" if "\<forall>x \<in> (set xs). HML_simulation x"
+trace: "HML_failure (hml_pos \<alpha> \<phi>)" if "HML_failure \<phi>" |
+neg: "HML_failure (hml_conj {} \<psi>s J n\<psi>s)" 
+    if "\<forall>j \<in> J. \<exists>\<alpha>. ((n\<psi>s j) = hml_pos \<alpha> TT \<or> (\<exists>\<chi>s n\<chi>s. (n\<psi>s j) = hml_pos \<alpha> (hml_conj {} \<chi>s {} n\<chi>s)))" 
+
+inductive HML_simulation :: "('a, 's)hml \<Rightarrow> bool"
+  where
+sim_pos: "HML_simulation (hml_pos \<alpha> \<phi>)" if "HML_simulation \<phi>"|
+sim_conj: "HML_simulation (hml_conj xs [])" if "\<forall>x \<in> (set xs). HML_simulation x"
 
 definition HML_simulation_formulas where
 "HML_simulation_formulas \<equiv> {\<phi>. HML_simulation \<phi>}"
 
-inductive HML_readiness :: "('a)formula_list \<Rightarrow> bool"
+inductive HML_readiness :: "('a, 's)hml \<Rightarrow> bool"
   where
 read_pos: "HML_readiness (HML_poss \<alpha> \<phi>)" if "HML_readiness \<phi>"|
 read_conj: "HML_readiness (HML_conj xs ys)" 
@@ -155,5 +178,5 @@ inductive HML_revivals :: "('a) formula_list \<Rightarrow> bool"
 revivals_pos: "HML_revivals (HML_poss \<alpha> \<phi>)" if "HML_revivals \<phi>" |
 revivals_conj: "HML_revivals (HML_conj xs ys)" if "\<exists>\<alpha>. \<forall>x \<in> set xs. x = HML_poss \<alpha> (HML_conj [] []) \<and>
 (\<forall>x \<in> set ys. \<exists>\<alpha>. x = HML_poss \<alpha> (HML_conj [] []))"
-
+*)
 end
